SystemF2Data: work on splitting lits from prims
Ignore-this: 3bae96aa23e30403f166338fcdd9fa5a

darcs-hash:20130424064404-08f32-a0d634d6b07ae5038fbd7c2865b64d9c5a6abed7

done/Iron/Language/SystemF2Data/Exp/Relation/WnfX.v
@@ -21,7 +21,16 @@ Inductive wnfX : exp -> Prop :=
  | Wnf_XCon
    :  forall dc ts xs
    ,  Forall wnfX xs
-   -> wnfX (XCon dc ts xs).
+   -> wnfX (XCon dc ts xs)
+
+ (* Literals are always wnf. *)
+ | Wnf_XPrim_PNat
+   :  forall n
+   ,  wnfX (XPrim (PNat n) nil)
+
+ | Wnf_XPrim_PBool
+   :  forall b
+   ,  wnfX (XPrim (PBool b) nil).
 Hint Constructors wnfX.
 
 
