done/Iron/Language/SystemF2Data/Exp/Lit.v
@@ -1,0 +1,9 @@
+
+
+Inductive lit : Type :=
+ (* Literal natural number. *)
+ | LNat   : nat  -> lit
+
+ (* Literal boolean. *)
+ | Bool   : bool -> lit.
+
