done/Iron/Language/SystemF2Data/Step/Step.v
@@ -3,12 +3,24 @@ Require Export Iron.Language.SystemF2Data.Exp.
 Require Export Iron.Language.SystemF2Data.Step.Context.
 
 
+(* Single step evaluation for primitives. *)
+Fixpoint primStep (p : prim) (xs : list exp) : option exp :=
+ match p, xs with
+ |  PAdd,    XPrim (PNat n1) nil :: XPrim (PNat n2) nil :: nil 
+ => Some (XPrim (PNat (n1 + n2)) nil)
+
+ |  PIsZero, XPrim (PNat n1) nil :: nil
+ => Some (XPrim (PBool (if beq_nat n1 0 then true else false)) nil)
+
+ | _, _
+ => None
+ end.
+
+
 (** * Single Small Step Evaluation *)
 (** The single step rules model the individual transitions that the 
      machine can make at runtime. *)
-
 Inductive STEP : exp -> exp -> Prop :=
-
  (* Step some sub-expression in an evaluation context *)
  | EsContext 
    :  forall C x x'
@@ -16,24 +28,33 @@ Inductive STEP : exp -> exp -> Prop :=
    -> STEP x x'
    -> STEP (C x) (C x')
 
+ (* Function application. *)
  | EsLamApp
    : forall t11 x12 v2
    ,  wnfX v2
    -> STEP (XApp   (XLam t11 x12) v2)
            (substXX 0 v2 x12)
 
- (* type applications *)
+ (* Type application. *)
  | EsLAMAPP
    :  forall x12 t2      
    ,  STEP (XAPP (XLAM x12) t2)
            (substTX 0 t2 x12)
 
+ (* Case branching. *)
  | EsCaseAlt
    :  forall dc ts vs alts x
    ,  Forall wnfX vs
    -> getAlt dc alts = Some (AAlt dc x)
    -> STEP (XCase (XCon dc ts vs) alts)
-           (substXXs 0 vs x).
+           (substXXs 0 vs x)
+
+ (* Primitives. *)
+ | EsPrim
+   :  forall p vs vResult
+   ,  Forall wnfX vs
+   -> primStep p vs = Some vResult
+   -> STEP (XPrim p vs) vResult.
 
 Hint Constructors STEP.
 
@@ -45,19 +66,42 @@ Lemma step_wnfX
 Proof.
  intros x v HW HS.
  induction HS; nope.
-  destruct H; auto; nope.
 
- Case "XCon dc (C x)".
-  inverts HW.
-  assert (wnfX x).
-  eapply exps_ctx_Forall; eauto.
-  assert (x' = x); auto.
-  subst. auto.
+ - Case "Step in context".
+   destruct H; auto; nope.
+
+   + SCase "XPrim".
+     inverts HW; inverts H; nope.
+
+   + SCase "XCon".
+     inverts HW.
+     have (wnfX x)
+      by (eapply exps_ctx_Forall; eauto).
+     have (x' = x).
+     subst. auto.
+
+ - Case "XPrim steps".
+   destruct p;
+    try (solve [simpl in H0; snorm]).
+   * inverts HW.
+   * inverts HW.
+Qed.
+
+
+Lemma step_context_XPrim_exists
+ :  forall C x p
+ ,  exps_ctx wnfX C
+ -> (exists x', STEP x x')
+ -> (exists x', STEP (XPrim p (C x)) (XPrim p (C x'))).
+Proof.
+ intros C x p HC HS.
+ shift x'.
+ eapply (EsContext (fun xx => XPrim p (C xx))); auto.
 Qed.
 
 
 Lemma step_context_XCon_exists
- :  forall  C x dc ts
+ :  forall C x dc ts
  ,  exps_ctx wnfX C 
  -> (exists x', STEP x x')
  -> (exists x', STEP (XCon dc ts (C x)) (XCon dc ts (C x'))).
@@ -66,5 +110,4 @@ Proof.
  shift x'.
  eapply (EsContext (fun xx => XCon dc ts (C xx))); auto.
 Qed.
-
 
